theories/sim/local.v
@@ -6,7 +6,7 @@ From stbor.lang Require Import defs.
 Set Default Proof Using "Type".
 
 Definition never_stuck fs e σ :=
-  ∀ e' σ', (e, σ) ~{fs}~>* (e', σ') → terminal e' ∨ reducible (Λ:=bor_lang fs)  e' σ'.
+  ∀ e' σ', (e, σ) ~{fs}~>* (e', σ') → terminal e' ∨ reducible fs e' σ'.
 
 Section local.
 Context {A: ucmraT}.
@@ -69,7 +69,7 @@ Inductive _sim_local_body_step (r_f : A) (sim_local_body : SIM)
 Record sim_local_body_base (r_f: A) (sim_local_body : SIM)
   (r: A) (idx: nat) es σs et σt Φ : Prop := {
   sim_local_body_stuck :
-    (terminal et ∨ reducible (Λ:= bor_lang fnt) et σt) ;
+    (terminal et ∨ reducible fnt et σt) ;
   sim_local_body_terminal :
     (* if tgt is terminal *)
     ∀ vt (TERM: to_result et = Some vt),
